fairis/heap_lang/examples/even_odd/model_updates.v
@@ -9,84 +9,13 @@ From trillium.program_logic Require Export weakestpre.
 From trillium.fairness Require Import fairness fair_termination utils action_model fuel resources.
 From trillium.fairness.heap_lang Require Export lang lifting tactics proofmode iris_inst.
 From trillium.fairness.heap_lang Require Import notation.
+From trillium.fairness.heap_lang.examples Require Import env_am split_model.
 From trillium.fairness.heap_lang.examples.even_odd Require Import interface thread_progs mu_role.
 Import derived_laws_later.bi.
 
 Open Scope nat.
 
 Set Default Proof Using "Type".
-
-
-Section SplitModel.
-  Let factor_repr (AM: ActionModel) := optionUR $ exclR $ leibnizO (amSt AM).
-
-  Let split_cmra (AM1 AM2: ActionModel) := (authUR $ prodUR (factor_repr AM1) (factor_repr AM2)). 
-  Definition SplitΣ (AM1 AM2: ActionModel) : gFunctors :=
-    #[GFunctor (split_cmra AM1 AM2)].
-
-  Class SplitPreGS Σ (AM1 AM2: ActionModel) := {
-      spre_in :> inG Σ (split_cmra AM1 AM2);
-  }.
-
-  Class SplitGS Σ (AM1 AM2: ActionModel) := {
-      spre :> SplitPreGS Σ AM1 AM2;
-      γ__split: gname;
-  }.
-
-  Lemma split_init `{SplitPreGS Σ AM1 AM2} st1 st2:
-    ⊢ |==> ∃ γ, own γ (● (Excl' st1, Excl' st2)) ∗
-           own γ (◯ (Excl' st1, None)) ∗ own γ (◯ (None, Excl' st2)).
-  Proof. 
-    iMod (own_alloc (● (Excl' st1, Excl' st2) ⋅ ◯ _)) as (γ) "[AUTH FRAG]".
-    { by apply auth_both_valid_2. }
-    iFrame. rewrite -own_op -auth_frag_op -pair_op. by iFrame.
-  Qed. 
-
-  Context {AM1 AM2: ActionModel}.
-  Context `{SplitGS Σ AM1 AM2}.
-
-  Let PM := ProdAM AM1 AM2.
-  Context `{AM_strong_lr PM}.
-  Let M := AM2FM PM _. 
-
-  Context {LM: LiveModel heap_lang M}. 
-  
-  Context {hGS: heapGS Σ LM}. 
-
-  Definition frag_left_st_is (st: amSt AM1): iProp Σ :=
-    own γ__split (◯ ((Excl' st, None): prodUR (factor_repr AM1) _)). 
-  Definition frag_right_st_is (st: amSt AM2): iProp Σ :=
-    own γ__split (◯ ((None, Excl' st): prodUR _ (factor_repr AM2))). 
-  Definition auth_prod_st_is st1 st2: iProp Σ :=
-    own γ__split (● ((Excl' st1, Excl' st2): prodUR _ (factor_repr AM2))). 
-
-  Lemma update_left (δ δ1 δ2: amSt AM1) (δ': amSt AM2):
-    auth_prod_st_is δ1 δ' -∗ frag_left_st_is δ2 ==∗ auth_prod_st_is δ δ' ∗ frag_left_st_is δ.
-  Proof.
-    iIntros "H1 H2". iCombine "H1 H2" as "H".
-    iMod (own_update with "H") as "[??]"; eauto.
-    2: { rewrite bi.sep_comm. by iFrame. } 
-    simpl. apply auth_update.
-    eapply @prod_local_update_1.
-    eapply @option_local_update.
-    by apply (exclusive_local_update _ ((Excl δ): exclR $ leibnizO (amSt AM1))).
-  Qed.
-
-  Lemma left_agree s1 s2 s':
-    auth_prod_st_is s1 s' -∗ frag_left_st_is s2 -∗ ⌜ s1 = s2 ⌝.
-  Proof.
-    iIntros "Ha Hf".
-    iDestruct (own_valid_2 with "Ha Hf") as %[SUB ?]%auth_both_valid_discrete.
-    apply pair_included in SUB as [SUB _]. simpl in SUB.
-    by apply @Excl_included, leibniz_equiv in SUB.
-  Qed.
-
-  Definition split_inv_inner: iProp Σ :=
-    ∃ st__G, frag_model_is st__G ∗ auth_prod_st_is st__G.1 st__G.2. 
-
-  Definition split_inv Ns := inv Ns split_inv_inner.
-
-End SplitModel.
 
 
 Section Models.
@@ -109,18 +38,6 @@ Section Models.
      Even the interface lemmas don't seem enough *)
   (* Global Instance prod_AM_act_dec: ∀ a : Action, Decision (is_action_of prod_model a). *)
   Context {prod_AM_act_dec: ∀ a, Decision (is_action_of prod_model a)}. 
-
-  Class EnvironmentAM (env_AM: ActionModel) := {
-      (* eam_role_eqdec :> EqDecision (amRole env_AM); *)
-      (* eam_role_cnt :> Countable (amRole env_AM); *)
-      eam_st_eqdec :> EqDecision (amSt env_AM);
-      eam_st_inh :> Inhabited (amSt env_AM);
-      eam_env_fb :> AM_fin_branch' env_AM;
-      eam_act_dec :> ∀ a, Decision (is_action_of env_AM a);
-      eam_step_dec :> AM_step_dec env_AM;
-  }.
-  Existing Instance eam_env_fb.
-  Existing Instance eam_step_dec. 
 
   Context `(ENV_AM: EnvironmentAM env_AM).
 
