fairis/heap_lang/examples/env_am.v
@@ -1,0 +1,22 @@
+From trillium.fairness Require Import action_model.
+From stdpp Require Import base. 
+From trillium.fairness Require Import utils.
+From iris.proofmode Require Import proofmode.
+
+Class EnvironmentAM (env_AM: ActionModel) := {
+    (* eam_role_eqdec :> EqDecision (amRole env_AM); *)
+    (* eam_role_cnt :> Countable (amRole env_AM); *)
+    eam_st_eqdec :> EqDecision (amSt env_AM);
+    eam_st_inh :> Inhabited (amSt env_AM);
+    eam_env_fb :> AM_fin_branch' env_AM;
+    eam_act_dec :> forall a, Decision (is_action_of env_AM a);
+    eam_step_dec :> AM_step_dec env_AM;
+  }.
+Existing Instance eam_env_fb.
+Existing Instance eam_step_dec.
+
+Instance EnvUnitAM: EnvironmentAM UnitAM.
+Proof. 
+  unshelve esplit.
+  all: by apply _.
+Defined.
