fairis/heap_lang/examples/even_odd/eo_vs_mod.v
@@ -9,6 +9,7 @@ From trillium.program_logic Require Export weakestpre.
 From trillium.fairness Require Import fairness fair_termination utils action_model resources.
 From trillium.fairness.heap_lang Require Export lang lifting tactics proofmode.
 From trillium.fairness.heap_lang Require Import notation sswp_rules iris_inst.
+From trillium.fairness.heap_lang.examples Require Import env_am split_model.
 From trillium.fairness.heap_lang.examples.even_odd Require Import interface thread_progs model_updates.
 Import derived_laws_later.bi.
 
